WIP SimplerSafeProtocol

protocols/SimplerSafeProtocol.v
@@ -1,34 +1,44 @@
 (* DISTRIBUTION STATEMENT A. Approved for public release. Distribution is unlimited.
  *
- * This material is based upon work supported by the Department of the Air Force under Air Force 
- * Contract No. FA8702-15-D-0001. Any opinions, findings, conclusions or recommendations expressed 
- * in this material are those of the author(s) and do not necessarily reflect the views of the 
+ * This material is based upon work supported by the Department of the Air Force under Air Force
+ * Contract No. FA8702-15-D-0001. Any opinions, findings, conclusions or recommendations expressed
+ * in this material are those of the author(s) and do not necessarily reflect the views of the
  * Department of the Air Force.
- * 
+ *
  * © 2019 Massachusetts Institute of Technology.
- * 
+ *
  * MIT Proprietary, Subject to FAR52.227-11 Patent Rights - Ownership by the contractor (May 2014)
- * 
+ *
  * The software/firmware is provided to you on an As-Is basis
- * 
+ *
  * Delivered to the U.S. Government with Unlimited Rights, as defined in DFARS Part 252.227-7013
  * or 7014 (Feb 2014). Notwithstanding any copyright notice, U.S. Government rights in this work are
  * defined by DFARS 252.227-7013 or DFARS 252.227-7014 as detailed above. Use of this work other than
  * as specifically authorized by the U.S. Government may violate any copyrights that exist in this work. *)
 
 From Coq Require Import
-     List.
+     List
+     JMeq.
 
-Require Import
-        MyPrelude
-        Maps
-        Keys
-        Messages
-        Tactics
-        Simulation
-        RealWorld
-        AdversarySafety
-        ProtocolAutomation.
+From KeyManagement Require Import
+     MyPrelude
+     Common
+     ProtocolAutomation
+     Automation
+     Maps
+     Keys
+     Messages
+     Tactics
+     Simulation
+     RealWorld
+     AdversarySafety.
+
+From protocols Require Import
+     SafeProtocol
+     (* Sets *)
+     ProtocolAutomation.
+
+From protocols Require Sets.
 
 Require IdealWorld.
 
@@ -51,10 +61,1329 @@ Section RealWorldLemmas.
     destruct lbl;
       intuition eauto.
 
-    unfold adv_universe_ok in *; split_ands; 
+    unfold adv_universe_ok in *; split_ands;
       eapply honest_labeled_step_univ_ok;
       eauto using honest_cmds_implies_safe_actions.
   Qed.
+
+  (* Partial order reduction *)
+
+  Inductive nextAction : forall {A B}, user_cmd A -> user_cmd B -> Prop :=
+  | NaReturn : forall A (a : << A >>),
+      nextAction (Return a) (Return a)
+  | NaGen :
+      nextAction Gen Gen
+  | NaSend : forall t uid (msg : crypto t),
+      nextAction (Send uid msg) (Send uid msg)
+  | NaRecv : forall t pat,
+      nextAction (@Recv t pat) (@Recv t pat)
+  | NaSignEncrypt : forall t k__s k__e u_id (msg : message t),
+      nextAction (SignEncrypt k__s k__e u_id msg) (SignEncrypt k__s k__e u_id msg)
+  | NaDecrypt : forall t (msg : crypto t),
+      nextAction (Decrypt msg) (Decrypt msg)
+  | NaSign : forall t k u_id (msg : message t),
+      nextAction (Sign k u_id msg) (Sign k u_id msg)
+  | NaVerify : forall t k (msg : crypto t),
+      nextAction (Verify k msg) (Verify k msg)
+  | NaGenSymKey : forall usg,
+      nextAction (GenerateSymKey usg) (GenerateSymKey usg)
+  | NaGenAsymKey : forall usg,
+      nextAction (GenerateAsymKey usg) (GenerateAsymKey usg)
+  | NaBind : forall A B r (c : user_cmd B) (c1 : user_cmd r) (c2 : << r >> -> user_cmd A),
+      nextAction c1 c
+      -> nextAction (Bind c1 c2) c
+  .
+
+  Record summary := { sending_to : Sets.set user_id }.
+
+  Inductive summarize : forall {t}, user_cmd t -> summary -> Prop :=
+  | SumReturn : forall t r s,
+      summarize (@Return t r) s
+  | SumGen : forall s,
+      summarize Gen s
+  | SumSend : forall {t} (msg : crypto t) uid s,
+      Sets.In uid s.(sending_to)
+      -> summarize (Send uid msg) s
+  | SumRecv : forall t pat s,
+      summarize (@Recv t pat) s
+  | SumSignEncrypt : forall t k__s k__e u_id (msg : message t)s ,
+      summarize (SignEncrypt k__s k__e u_id msg) s
+  | SumDecrypt : forall t (msg : crypto t) s,
+      summarize (Decrypt msg) s
+  | SumSign : forall t k u_id (msg : message t) s,
+      summarize (Sign k u_id msg) s
+  | SumVerify : forall t k (msg : crypto t) s,
+      summarize (Verify k msg) s
+  | SumGenSymKey : forall usg s,
+      summarize (GenerateSymKey usg) s
+  | SumGenAsymKey : forall usg s,
+      summarize (GenerateAsymKey usg) s
+  | SumBind : forall t1 t2 (c1 : user_cmd t1) (c2 : << t1 >> -> user_cmd t2) s,
+      summarize c1 s
+      -> (forall r__v, summarize (c2 r__v) s)
+      -> summarize (Bind c1 c2) s
+  .
+
+  Definition commutes {t} (cmd : user_cmd t) (s : summary) : Prop :=
+    match cmd with
+    | Return _ => True
+    | Gen => True
+    | Send uid _ => False (* For now, be imprecise ~ uid \in s.(sending_to) *)
+    | Recv _ => True
+    | SignEncrypt _ _ _ _ => True
+    | Decrypt _ => True
+    | Sign _ _ _ => True
+    | Verify _ _ => True
+    | GenerateSymKey _ => True
+    | GenerateAsymKey _ => True
+    | Bind _ _ => False
+    end.
+
+  Definition hstep {A B} (lbl : rlabel) (suid : option user_id) (bd bd' : data_step0 A B (Base A)) :=
+    step_user lbl suid bd bd'.
+
+  Lemma step_na_return :
+    forall {A B C D} suid lbl bd bd',
+
+      step_user lbl suid bd bd'
+
+      -> forall cs cs' (usrs usrs': honest_users A) (adv adv' : user_data B) gks gks'
+          (cmd cmd' : user_cmd C) ks ks' qmsgs qmsgs' mycs mycs'
+          froms froms' sents sents' cur_n cur_n' r,
+
+        bd = (usrs, adv, cs, gks, ks, qmsgs, mycs, froms, sents, cur_n, cmd)
+        -> bd' = (usrs', adv', cs', gks', ks', qmsgs', mycs', froms', sents', cur_n', cmd')
+        -> @nextAction C D cmd (Return r)
+        -> usrs = usrs'
+        /\ adv = adv'
+        /\ cs = cs'
+        /\ gks = gks'
+        /\ ks = ks'
+        /\ qmsgs = qmsgs'
+        /\ mycs = mycs'
+        /\ froms = froms'
+        /\ sents = sents'
+        /\ cur_n = cur_n'.
+
+  Proof.
+    induction 1; inversion 1; inversion 1; intros; subst;
+      match goal with
+      | [ H : nextAction _ _ |- _ ] => invert H
+      end; eauto.
+
+    intuition idtac.
+  Qed.
+
+  Lemma step_na_not_return :
+    forall {A B C D} suid lbl bd bd',
+
+      step_user lbl suid bd bd'
+
+      -> forall cs cs' (usrs usrs': honest_users A) (adv adv' : user_data B) gks gks'
+          (cmd cmd' : user_cmd C) (cmd__n : user_cmd D) ks ks' qmsgs qmsgs' mycs mycs'
+          froms froms' sents sents' cur_n cur_n',
+
+        bd = (usrs, adv, cs, gks, ks, qmsgs, mycs, froms, sents, cur_n, cmd)
+        -> bd' = (usrs', adv', cs', gks', ks', qmsgs', mycs', froms', sents', cur_n', cmd')
+        -> nextAction cmd cmd__n
+        -> (forall r, cmd__n <> Return r)
+        -> exists f cmd__n',
+            step_user lbl suid
+                      (usrs, adv, cs, gks, ks, qmsgs, mycs, froms, sents, cur_n, cmd__n)
+                      (usrs', adv', cs', gks', ks', qmsgs', mycs', froms', sents', cur_n', cmd__n')
+            /\ cmd = f cmd__n
+            /\ cmd' = f cmd__n'
+            /\ forall lbl1 suid1 (usrs1 usrs1' : honest_users A) (adv1 adv1' : user_data B)
+                cs1 cs1' gks1 gks1'
+                ks1 ks1' qmsgs1 qmsgs1' mycs1 mycs1' (cmd__n'' : user_cmd D)
+                froms1 froms1' sents1 sents1' cur_n1 cur_n1',
+
+                step_user lbl1 suid1
+                          (usrs1, adv1, cs1, gks1, ks1, qmsgs1, mycs1, froms1, sents1, cur_n1, cmd__n)
+                          (usrs1', adv1', cs1', gks1', ks1', qmsgs1', mycs1', froms1', sents1', cur_n1', cmd__n'')
+                -> step_user lbl1 suid1
+                            (usrs1, adv1, cs1, gks1, ks1, qmsgs1, mycs1, froms1, sents1, cur_n1, f cmd__n)
+                            (usrs1', adv1', cs1', gks1', ks1', qmsgs1', mycs1', froms1', sents1', cur_n1', f cmd__n'').
+  Proof.
+    Hint Constructors step_user.
+
+    induction 1; inversion 1; inversion 1; invert 1; intros.
+
+    - eapply IHstep_user in H28; eauto.
+      split_ex.
+      exists (fun CD => x <- x CD; cmd2 x).
+      eexists; subst; split; eauto.
+    - invert H27.
+      unfold not in *; exfalso; eauto.
+    - exists (fun x => x); eexists; repeat simple apply conj; swap 1 3; eauto.
+    - exists (fun x => x); eexists; repeat simple apply conj; swap 1 3; eauto.
+    - exists (fun x => x); eexists; repeat simple apply conj; swap 1 3; eauto.
+    - exists (fun x => x); eexists; repeat simple apply conj; swap 1 3; eauto.
+    - exists (fun x => x); eexists; repeat simple apply conj; swap 1 3; eauto.
+    - exists (fun x => x); eexists; repeat simple apply conj; swap 1 3; eauto.
+    - exists (fun x => x); eexists; repeat simple apply conj; swap 1 3; eauto.
+    - exists (fun x => x); eexists; repeat simple apply conj; swap 1 3; eauto.
+    - exists (fun x => x); eexists; repeat simple apply conj; swap 1 3; eauto.
+    - exists (fun x => x); eexists; repeat simple apply conj; swap 1 3; eauto.
+  Qed.
+
+  Hint Constructors nextAction : core.
+  Definition data_step_no_cmd A B : Type :=
+    honest_users A * user_data B * ciphers * keys * key_perms * queued_messages * my_ciphers * recv_nonces * sent_nonces * nat.
+
+  Lemma step_implies_na :
+    forall {A B C} suid lbl bd bd',
+
+      step_user lbl suid bd bd'
+
+      (* -> forall cs cs' (usrs usrs': honest_users A) (adv adv' : user_data B) gks gks' *)
+      (*     (cmd cmd' : user_cmd C) ks ks' qmsgs qmsgs' mycs mycs' *)
+      (*     froms froms' sents sents' cur_n cur_n', *)
+        (*   bd = (usrs, adv, cs, gks, ks, qmsgs, mycs, froms, sents, cur_n, cmd) *)
+        (* -> bd' = (usrs', adv', cs', gks', ks', qmsgs', mycs', froms', sents', cur_n', cmd') *)
+      -> forall (bd__x bd__x' : data_step_no_cmd A B)  (cmd cmd' : user_cmd C),
+          bd = (bd__x, cmd)
+        -> bd' = (bd__x', cmd')
+        -> (exists R (r : <<R>>), @nextAction C R cmd (Return r))
+        \/ (exists D f (cmd__n cmd__n' : user_cmd D),
+              nextAction cmd cmd__n
+            /\ cmd = f cmd__n
+            /\ cmd' = f cmd__n'
+            /\ forall (bd__x1 bd__x1' : data_step_no_cmd A B),
+                 step_user lbl suid
+                          (bd__x1, cmd__n)
+                          (bd__x1', cmd__n')
+                -> step_user lbl suid
+                            (bd__x1, f cmd__n)
+                            (bd__x1', f cmd__n')
+
+          ).
+  Proof.
+    induction 1; inversion 1; inversion 1;
+      intros; subst; try solve [ right; eexists; exists (fun x => x); eauto 6]; eauto.
+
+    - specialize (IHstep_user _ _ _ _ eq_refl eq_refl).
+      split_ors; split_ex; subst.
+      + left; eauto 8.
+      + right; eexists; exists (fun CMD => x <- x0 CMD; cmd2 x);
+          (do 2 eexists); repeat simple apply conj; eauto; intros.
+        do 9 destruct bd__x1 as [bd__x1 ?x].
+        do 9 destruct bd__x1' as [bd__x1' ?x].
+        eapply StepBindRecur; eauto 12.
+  Qed.
+
+  Lemma nextAction_couldBe :
+    forall {A B} (c1 : user_cmd A) (c2 : user_cmd B),
+      nextAction c1 c2
+      -> match c2 with
+        | Return _ => True
+        | Gen => True
+        | Send _ _ => True
+        | Recv _ => True
+        | SignEncrypt _ _ _ _ => True
+        | Decrypt _ => True
+        | Sign _ _ _ => True
+        | Verify _ _ => True
+        | GenerateAsymKey _ => True
+        | GenerateSymKey _ => True
+        | Bind _ _ => False
+        end.
+  Proof.
+    induction 1; eauto.
+  Qed.
+
+  (* need to know that msg, if cipher, is in cs *)
+  (* Lemma findKeysCrypto_addnl_cipher : *)
+  (*   forall {t} (msg : crypto t) ks cs c_id c, *)
+  (*     ~ In c_id cs *)
+  (*     -> keys_mine ks (findKeysCrypto cs msg) *)
+  (*     -> findKeysCrypto cs msg = findKeysCrypto (cs $+ (c_id,c)) msg. *)
+  (* Proof. *)
+  (*   intros. *)
+  (*   unfold findKeysCrypto in *. *)
+  (*   destruct msg; eauto. *)
+  (*   destruct (c_id ==n c_id0); subst; clean_map_lookups; eauto. *)
+  (*   unfold keys_mine in H0. *)
+
+  (* need to know that msg, if cipher, is in cs *)
+  (* Lemma updateTrackedNonce_addnl_cipher : *)
+  (*   forall suid nons cs {t} (msg : crypto t) c_id c, *)
+  (*     ~ In c_id cs *)
+  (*     -> updateTrackedNonce suid nons cs msg = *)
+  (*       updateTrackedNonce suid nons (cs $+ (c_id, c)) msg. *)
+  (* Proof. *)
+  (*   intros. *)
+  (*   unfold updateTrackedNonce. *)
+  (*   destruct msg; eauto. *)
+  (*   destruct (c_id ==n c_id0); subst; clean_map_lookups.  *)
+
+  (* Lemma msg_not_accepted_pattern_addnl_cipher : *)
+  (*   forall {t} (msg : crypto t) cs suid froms pat c_id c, *)
+  (*     ~ In c_id cs *)
+  (*     -> ~ msg_accepted_by_pattern cs suid froms pat msg *)
+  (*     -> ~ msg_accepted_by_pattern (cs $+ (c_id, c)) suid froms pat msg. *)
+  (* Proof. *)
+  (*   intros. *)
+  (*   unfold not. *)
+  (*   destruct pat; intros; eauto. *)
+  (*   - invert H1. *)
+
+  Lemma commutes_sound' :
+    forall {A B C D} suid1 u_id1 lbl1 (bd1 bd1' : data_step0 A B C),
+
+      step_user lbl1 suid1 bd1 bd1'
+      -> suid1 = Some u_id1
+      -> forall (bd2 bd2' : data_step0 A B D) lbl2 suid2 u_id2,
+
+          step_user lbl2 suid2 bd2 bd2'
+          -> suid2 = Some u_id2
+          -> u_id1 <> u_id2
+
+          -> forall cs cs1 cs' (usrs1 usrs1' usrs2 usrs2' : honest_users A) (adv adv1 adv' : user_data B) gks gks1 gks'
+              ks1 ks1' qmsgs1 qmsgs1' mycs1 mycs1' cmd1 cmd1' froms1 froms1' sents1 sents1' cur_n1 cur_n1'
+              ks2 ks2' qmsgs2 qmsgs2' mycs2 mycs2' cmd2 cmd2' froms2 froms2' sents2 sents2' cur_n2 cur_n2' s,
+
+                bd1  = (usrs1,  adv,  cs,  gks,  ks1, qmsgs1, mycs1, froms1, sents1, cur_n1, cmd1)
+              -> bd1' = (usrs1', adv1, cs1, gks1, ks1', qmsgs1', mycs1', froms1', sents1', cur_n1', cmd1')
+              -> bd2  = (usrs2,  adv1, cs1, gks1, ks2, qmsgs2, mycs2, froms2, sents2, cur_n2, cmd2)
+              -> bd2' = (usrs2', adv', cs', gks', ks2', qmsgs2', mycs2', froms2', sents2', cur_n2', cmd2')
+
+              (* no recursion *)
+              -> nextAction cmd1 cmd1
+              -> nextAction cmd2 cmd2
+              -> (forall cmd__n x t (m : crypto t), nextAction cmd1 cmd__n -> cmd__n <> Send x m)
+
+              -> summarize cmd1 s
+              -> commutes cmd2 s
+
+              -> forall bd3 (usrs3 usrs4 : honest_users A),
+                  bd3 = (usrs3,   adv,  cs,  gks,  ks2, qmsgs2, mycs2, froms2, sents2, cur_n2, cmd2)
+                  -> exists bd3' bd4 bd4' lbl3 lbl4 adv2 cs2 gks2 usrs3' usrs4',
+                      step_user lbl3 suid2 bd3 bd3'
+                      /\ bd3' = (usrs3', adv2, cs2, gks2, ks2', qmsgs2', mycs2', froms2', sents2', cur_n2', cmd2')
+                      /\ bd4 = (usrs4,   adv2, cs2, gks2, ks1, qmsgs1, mycs1, froms1, sents1, cur_n1, cmd1)
+                      /\ bd4' = (usrs4', adv', cs', gks', ks1', qmsgs1', mycs1', froms1', sents1', cur_n1', cmd1')
+                      /\ step_user lbl4 suid1 bd4 bd4'
+  .
+  Proof.
+    intros;
+      cases cmd1; cases cmd2;
+      subst;
+      repeat
+        match goal with
+         | [ ARG : nextAction (Send ?u ?msg) (Send ?u ?msg) , H : (forall c _ _ _, nextAction (Send ?u ?msg) c -> c <> _) |- _ ] =>
+           specialize (H _ u _ msg ARG); contradiction
+        | [ H : nextAction ?c1 ?c2 |- _ ] => apply nextAction_couldBe in H; try contradiction
+        | [ H : commutes (Send _ _) _ |- _ ] => unfold commutes in H; contradiction
+        | [ H : step_user _ _ _ _ |- _ ] => invert H
+        end; subst;
+        churn;
+        try solve [ do 10 eexists; (repeat simple apply conj); try reflexivity; try econstructor; eauto; eauto ].
+
+    - do 10 eexists; (repeat simple apply conj); try reflexivity; try econstructor; eauto; eauto.
+         admit.
+    - do 10 eexists; (repeat simple apply conj); try reflexivity; try econstructor; eauto; eauto.
+         admit.
+    - do 10 eexists; (repeat simple apply conj); try reflexivity; try econstructor; eauto; eauto.
+         admit.
+    - do 10 eexists; (repeat simple apply conj); try reflexivity; try econstructor; eauto; eauto.
+         admit.
+    - do 10 eexists; (repeat simple apply conj); try reflexivity; try econstructor; eauto; eauto.
+         admit.
+         admit.
+
+    - do 10 eexists; (repeat simple apply conj); try reflexivity; try econstructor; eauto; eauto.
+         admit.
+    - do 10 eexists; (repeat simple apply conj); try reflexivity; try econstructor; eauto; eauto.
+         admit. admit. admit. admit.
+    - do 10 eexists; (repeat simple apply conj); try reflexivity; try econstructor; eauto; eauto.
+         admit.
+    - do 10 eexists; (repeat simple apply conj); try reflexivity; try econstructor; eauto; eauto.
+         admit.
+    - do 10 eexists; (repeat simple apply conj); try reflexivity; try econstructor; eauto; eauto.
+         admit.
+    - do 10 eexists; (repeat simple apply conj); try reflexivity; try econstructor; eauto; eauto.
+         admit.
+    - do 10 eexists; (repeat simple apply conj); try reflexivity; try econstructor; eauto; eauto.
+         admit.
+    - do 10 eexists; (repeat simple apply conj); try reflexivity; try econstructor; eauto; eauto.
+         admit.
+    - do 10 eexists; (repeat simple apply conj); try reflexivity; try econstructor; eauto; eauto.
+         admit. admit.
+    - do 10 eexists; (repeat simple apply conj); try reflexivity; try econstructor; eauto; eauto.
+         admit. admit. admit. 
+    - do 10 eexists; (repeat simple apply conj); try reflexivity; try econstructor; eauto; eauto.
+         admit.
+         (* ~ msg_accepted_by_pattern cs1 (Some u_id1) froms1 pat msg0 *)
+         (*   ===================== *)
+         (*   ~ msg_accepted_by_pattern (cs1 $+ (c_id, SigEncCipher k__sign k__enc msg_to (Some u_id2, cur_n2) msg)) (Some u_id1) froms1 pat msg0 *)
+         admit.
+    - do 10 eexists; (repeat simple apply conj); try reflexivity; try econstructor; eauto; eauto.
+         admit.
+    - do 10 eexists; (repeat simple apply conj); try reflexivity; try econstructor; eauto; eauto.
+         admit. admit. admit.
+    - do 10 eexists; (repeat simple apply conj); try reflexivity; try econstructor; eauto; eauto.
+         admit. admit.
+    - do 10 eexists; (repeat simple apply conj); try reflexivity; try econstructor; eauto; eauto.
+         admit.
+    - do 10 eexists; (repeat simple apply conj); try reflexivity; try econstructor; eauto; eauto.
+         admit.
+    - do 10 eexists; (repeat simple apply conj); try reflexivity; try econstructor; eauto; eauto.
+         admit.
+    - do 10 eexists; (repeat simple apply conj); try reflexivity; try econstructor; eauto; eauto.
+         admit.
+    - do 10 eexists; (repeat simple apply conj); try reflexivity; try econstructor; eauto; eauto.
+         admit.
+    - do 10 eexists; (repeat simple apply conj); try reflexivity; try econstructor; eauto; eauto.
+         admit.
+    - do 10 eexists; (repeat simple apply conj); try reflexivity; try econstructor; eauto; eauto.
+         admit.
+    - do 10 eexists; (repeat simple apply conj); try reflexivity; try econstructor; eauto; eauto.
+         admit.
+    - do 10 eexists; (repeat simple apply conj); try reflexivity; try econstructor; eauto; eauto.
+         admit.
+    - do 10 eexists; (repeat simple apply conj); try reflexivity; try econstructor; eauto; eauto.
+         admit.
+    - do 10 eexists; (repeat simple apply conj); try reflexivity; try econstructor; eauto; eauto.
+         admit.
+    - do 10 eexists; (repeat simple apply conj); try reflexivity; try econstructor; eauto; eauto.
+         admit.
+    - do 10 eexists; (repeat simple apply conj); try reflexivity; try econstructor; eauto; eauto.
+         admit.
+    - do 10 eexists; (repeat simple apply conj); try reflexivity; try econstructor; eauto; eauto.
+         admit.
+    - do 10 eexists; (repeat simple apply conj); try reflexivity; try econstructor; eauto; eauto.
+         admit.
+    - do 10 eexists; (repeat simple apply conj); try reflexivity; try econstructor; eauto; eauto.
+         admit.
+    - do 10 eexists; (repeat simple apply conj); try reflexivity; try econstructor; eauto; eauto.
+         admit.
+    - do 10 eexists; (repeat simple apply conj); try reflexivity; try econstructor; eauto; eauto.
+         admit.
+    - do 10 eexists; (repeat simple apply conj); try reflexivity; try econstructor; eauto; eauto.
+         admit.
+    - do 10 eexists; (repeat simple apply conj); try reflexivity; try econstructor; eauto; eauto.
+         admit.
+    - do 10 eexists; (repeat simple apply conj); try reflexivity; try econstructor; eauto; eauto.
+         admit.
+    - do 10 eexists; (repeat simple apply conj); try reflexivity; try econstructor; eauto; eauto.
+         admit.
+       
+
+
+    
+    Ltac p :=
+      match goal with
+      | [ |- _ /\ _ ] => simple apply conj
+      | [ |- _ = _ ] => reflexivity
+      | [ |- step_user _ _ _ _ ] => solve [ econstructor; repeat p; eauto ]
+      | [ H : ?m $+ (?k1,_) $? ?k2 = None |- ?m $? ?k3 = None ] =>
+        match type of m with
+        | keys => idtac
+        | ciphers => idtac
+        end;
+        is_not_evar k1; is_not_evar k2; is_evar k3; unify k3 k2;
+          destruct (k1 ==n k2); subst; clean_map_lookups; idtac 1
+      | [ H : ?m $+ (?k1,_) $? ?k2 = None |- ?m $+ (?k2,_) $? ?k3 = None ] =>
+        match type of m with
+        | keys => idtac
+        | ciphers => idtac
+        end;
+        is_not_evar k1; is_not_evar k2; is_evar k3; unify k3 k1;
+          destruct (k1 ==n k2); subst; clean_map_lookups; idtac 2
+      | [ |- (_,_) = _ ] => f_equal
+      | [ |- _ $+ (_,_) = _ ] => maps_equal
+      | [ |- _ $+ (_,_) $? _ = _ ] => clean_map_lookups
+      end.
+
+    Ltac simpl_solve uid :=
+      split_ex; subst;
+      match goal with
+      | [ H : step_user _ (Some uid) _ _ |- _ ] => invert H; try contradiction
+      end; clean_map_lookups;
+      do 29 eexists;
+         repeat p;
+         eauto;
+         repeat
+           match goal with
+           | [ |- hstep _ _ _ _ ] => solve [ econstructor; eauto ]
+           | [ H : forall _ _ _ _ _ _ _ _ _ _ _ _ _ _ _ _ _ _ _ _ _ _ _, step_user _ _ _ _  -> step_user _ _ _ _ |- hstep _ _ _ _ ] =>
+             solve [ eapply H; eauto ] 
+           end.
+         
+    induction 1; inversion 5; inversion 1; intros;
+      clean_context;
+      repeat 
+        match goal with
+        | [ H : (_,_,_,_,_,_,_,_,_,_,_) = (_,_,_,_,_,_,_,_,_,_,_) |- _ ] => invert H
+        | [ H : commutes _ _ |- _ ] => unfold commutes in H; try contradiction
+        end; clean_context; try (solve [ simpl_solve u_id2 ] ).
+
+
+    - apply nextAction_couldBe in H30; contradiction.
+    - split_ex; subst.
+      match goal with
+      | [ H : step_user _ (Some u_id2) _ _ |- _ ] => invert H; try contradiction
+      end; clean_map_lookups.
+      + destruct (rec_u_id ==n u_id2); subst; clean_map_lookups; simpl in *.
+        * do 29 eexists; repeat p; eauto.
+             econstructor; eauto.
+             eapply H5; eauto.
+             invert H40.
+             econstructor; eauto.
+        * do 29 eexists; repeat p; eauto.
+             econstructor; eauto.
+             eapply H5; eauto.
+             invert H40.
+             econstructor; eauto.
+             clean_map_lookups.
+             reflexivity.
+      + destruct (rec_u_id ==n u_id2); subst; clean_map_lookups; simpl in *.
+        * do 29 eexists; repeat p; eauto.
+             econstructor; eauto.
+             eapply H5; eauto.
+             invert H40.
+             econstructor; eauto.
+        * do 29 eexists; repeat p; eauto.
+             econstructor; eauto.
+             eapply H5; eauto.
+             invert H40.
+             econstructor; eauto.
+             clean_map_lookups.
+           reflexivity.
+
+      + destruct (rec_u_id ==n u_id2); subst; clean_map_lookups; simpl in *.
+        * do 29 eexists; repeat p; eauto.
+             econstructor; eauto.
+             eapply H5; eauto.
+             invert H40.
+             econstructor; eauto.
+        * do 29 eexists; repeat p; eauto.
+             econstructor; eauto.
+             eapply H5; eauto.
+             invert H40.
+             econstructor; eauto.
+             clean_map_lookups.
+           reflexivity.
+
+    - split_ex; subst.
+      match goal with
+      | [ H : step_user _ (Some u_id2) _ _ |- _ ] => invert H; try contradiction
+      end; clean_map_lookups.
+      + do 29 eexists; repeat p; eauto.
+           econstructor; eauto.
+           eapply H2; eauto.
+      + do 29 eexists; repeat p; eauto.
+           destruct (k_id ==n k_id0); subst; econstructor; eauto.
+           eapply H2; eauto.
+      + do 29 eexists; repeat p; eauto.
+           destruct (k_id ==n k_id0); subst; econstructor; eauto.
+           eapply H2; eauto.
+
+    - split_ex; subst.
+      match goal with
+      | [ H : step_user _ (Some u_id2) _ _ |- _ ] => invert H; try contradiction
+      end; clean_map_lookups.
+      + do 29 eexists; repeat p; eauto.
+           econstructor; eauto.
+           eapply H2; eauto.
+      + do 29 eexists; repeat p; eauto.
+           destruct (k_id ==n k_id0); subst; econstructor; eauto.
+           eapply H2; eauto.
+      + do 29 eexists; repeat p; eauto.
+           destruct (k_id ==n k_id0); subst; econstructor; eauto.
+           eapply H2; eauto.
+  Qed.
+  Lemma commutes_sound' :
+    forall {A B C} suid1 u_id1 lbl1 (bd1 bd1' : data_step0 A B C),
+
+      step_user lbl1 suid1 bd1 bd1'
+      -> suid1 = Some u_id1
+      -> forall bd2 bd2' lbl2 suid2 u_id2,
+
+          step_user lbl2 suid2 bd2 bd2'
+          -> suid2 = Some u_id2
+          -> u_id1 <> u_id2
+
+          -> forall cs1 cs1' cs1'' (usrs1 usrs1': honest_users A) (adv1 adv1' adv1'' : user_data B) gks1 gks1' gks1''
+              (cmd__n1 cmd__n1' : user_cmd C) ks1 ks1' qmsgs1 qmsgs1' mycs1 mycs1'
+              (cmd1 cmd1' cmd2 cmd2': user_cmd (Base A))
+              froms1 froms1' sents1 sents1' cur_n1 cur_n1'
+              usrs2 usrs2' ks2 ks2' qmsgs2 qmsgs2' mycs2 mycs2'
+              (* (cmd__n2 cmd__n2' : user_cmd D) *)
+              froms2 froms2' sents2 sents2' cur_n2 cur_n2' s,
+
+                bd1 = (usrs1, adv1, cs1, gks1, ks1, qmsgs1, mycs1, froms1, sents1, cur_n1, cmd__n1)
+              -> bd1' = (usrs1', adv1', cs1', gks1', ks1', qmsgs1', mycs1', froms1', sents1', cur_n1', cmd__n1')
+              -> bd2 = (usrs2, adv1', cs1', gks1', ks2, qmsgs2, mycs2, froms2, sents2, cur_n2, cmd2)
+              -> bd2' = (usrs2', adv1'', cs1'', gks1'', ks2', qmsgs2', mycs2', froms2', sents2', cur_n2', cmd2')
+
+              (* build link to overall user command *)
+              -> nextAction cmd1 cmd__n1
+              -> (forall r, cmd__n1 <> Return r)
+              -> (exists f, cmd1 = f cmd__n1
+                    /\ cmd1' = f cmd__n1'
+                     /\ forall lbl5 suid5 (usrs5 usrs5' : honest_users A) (adv5 adv5' : user_data B)
+                        cs5 cs5' gks5 gks5'
+                        ks5 ks5' qmsgs5 qmsgs5' mycs5 mycs5' (cmd__n'' : user_cmd C)
+                        froms5 froms5' sents5 sents5' cur_n5 cur_n5',
+
+                        step_user lbl5 suid5
+                                  (usrs5, adv5, cs5, gks5, ks5, qmsgs5, mycs5, froms5, sents5, cur_n5, cmd__n1)
+                                  (usrs5', adv5', cs5', gks5', ks5', qmsgs5', mycs5', froms5', sents5', cur_n5', cmd__n'')
+                        -> step_user lbl5 suid5
+                                    (usrs5, adv5, cs5, gks5, ks5, qmsgs5, mycs5, froms5, sents5, cur_n5, f cmd__n1)
+                                    (usrs5', adv5', cs5', gks5', ks5', qmsgs5', mycs5', froms5', sents5', cur_n5', f cmd__n'')
+
+                )
+              -> step_user lbl1 suid1
+                          (usrs1, adv1, cs1, gks1, ks1, qmsgs1, mycs1, froms1, sents1, cur_n1, cmd__n1)
+                          (usrs1', adv1', cs1', gks1', ks1', qmsgs1', mycs1', froms1', sents1', cur_n1', cmd__n1')
+
+              -> usrs1 $? u_id1 = Some (mkUserData ks1 cmd1 qmsgs1 mycs1 froms1 sents1 cur_n1)
+              -> usrs2 $? u_id2 = Some (mkUserData ks2 cmd2 qmsgs2 mycs2 froms2 sents2 cur_n2)
+              -> usrs2 = usrs1' $+ (u_id1, mkUserData ks1' cmd1' qmsgs1' mycs1' froms1' sents1' cur_n1')
+
+              -> summarize cmd1 s
+              -> commutes cmd2 s
+
+              -> forall bd3 ks3 qmsgs3 mycs3 froms3 sents3 cur_n3,
+                  bd3 = (usrs1, adv1, cs1, gks1, ks3, qmsgs3, mycs3, froms3, sents3, cur_n3, cmd2)
+                  -> usrs1 $? u_id2 = Some (mkUserData ks3 cmd2 qmsgs3 mycs3 froms3 sents3 cur_n3)
+                  
+                  -> exists bd3' lbl3 lbl4 bd4 bd4'
+                      cs3' (usrs3': honest_users A)
+                      (adv3' : user_data B) gks3'
+                      ks3' qmsgs3' mycs3' froms3' sents3' cur_n3'
+                      usrs4 usrs4' ks4 ks4' qmsgs4 qmsgs4' mycs4 mycs4'
+                      froms4 froms4' sents4 sents4' cur_n4 cur_n4',
+
+                      hstep lbl3 suid2 bd3 bd3'
+                      /\ bd3' = (usrs3', adv3', cs3', gks3', ks3', qmsgs3', mycs3', froms3', sents3', cur_n3', cmd2')
+                      /\ bd4 = (usrs4, adv3', cs3', gks3', ks4, qmsgs4, mycs4, froms4, sents4, cur_n4, cmd1)
+                      /\ bd4' = (usrs4', adv1'', cs1'', gks1'', ks4', qmsgs4', mycs4', froms4', sents4', cur_n4', cmd1')
+                      /\ usrs4 = usrs3' $+ (u_id2, mkUserData ks3' cmd2' qmsgs3' mycs3' froms3' sents3' cur_n3')
+                      /\ usrs4 $? u_id1 = Some (mkUserData ks4 cmd1 qmsgs4 mycs4 froms4 sents4 cur_n4)
+                      /\ hstep lbl4 suid1 bd4 bd4'
+  .
+  Proof.
+
+    Ltac p :=
+      match goal with
+      | [ |- _ /\ _ ] => simple apply conj
+      | [ |- _ = _ ] => reflexivity
+      | [ |- step_user _ _ _ _ ] => solve [ econstructor; repeat p; eauto ]
+      | [ H : ?m $+ (?k1,_) $? ?k2 = None |- ?m $? ?k3 = None ] =>
+        match type of m with
+        | keys => idtac
+        | ciphers => idtac
+        end;
+        is_not_evar k1; is_not_evar k2; is_evar k3; unify k3 k2;
+          destruct (k1 ==n k2); subst; clean_map_lookups; idtac 1
+      | [ H : ?m $+ (?k1,_) $? ?k2 = None |- ?m $+ (?k2,_) $? ?k3 = None ] =>
+        match type of m with
+        | keys => idtac
+        | ciphers => idtac
+        end;
+        is_not_evar k1; is_not_evar k2; is_evar k3; unify k3 k1;
+          destruct (k1 ==n k2); subst; clean_map_lookups; idtac 2
+      | [ |- (_,_) = _ ] => f_equal
+      | [ |- _ $+ (_,_) = _ ] => maps_equal
+      | [ |- _ $+ (_,_) $? _ = _ ] => clean_map_lookups
+      end.
+
+    Ltac simpl_solve uid :=
+      split_ex; subst;
+      match goal with
+      | [ H : step_user _ (Some uid) _ _ |- _ ] => invert H; try contradiction
+      end; clean_map_lookups;
+      do 29 eexists;
+         repeat p;
+         eauto;
+         repeat
+           match goal with
+           | [ |- hstep _ _ _ _ ] => solve [ econstructor; eauto ]
+           | [ H : forall _ _ _ _ _ _ _ _ _ _ _ _ _ _ _ _ _ _ _ _ _ _ _, step_user _ _ _ _  -> step_user _ _ _ _ |- hstep _ _ _ _ ] =>
+             solve [ eapply H; eauto ] 
+           end.
+         
+    induction 1; inversion 5; inversion 1; intros;
+      clean_context;
+      repeat 
+        match goal with
+        | [ H : (_,_,_,_,_,_,_,_,_,_,_) = (_,_,_,_,_,_,_,_,_,_,_) |- _ ] => invert H
+        | [ H : commutes _ _ |- _ ] => unfold commutes in H; try contradiction
+        end; clean_context; try (solve [ simpl_solve u_id2 ] ).
+
+
+    - apply nextAction_couldBe in H30; contradiction.
+    - split_ex; subst.
+      match goal with
+      | [ H : step_user _ (Some u_id2) _ _ |- _ ] => invert H; try contradiction
+      end; clean_map_lookups.
+      + destruct (rec_u_id ==n u_id2); subst; clean_map_lookups; simpl in *.
+        * do 29 eexists; repeat p; eauto.
+             econstructor; eauto.
+             eapply H5; eauto.
+             invert H40.
+             econstructor; eauto.
+        * do 29 eexists; repeat p; eauto.
+             econstructor; eauto.
+             eapply H5; eauto.
+             invert H40.
+             econstructor; eauto.
+             clean_map_lookups.
+             reflexivity.
+      + destruct (rec_u_id ==n u_id2); subst; clean_map_lookups; simpl in *.
+        * do 29 eexists; repeat p; eauto.
+             econstructor; eauto.
+             eapply H5; eauto.
+             invert H40.
+             econstructor; eauto.
+        * do 29 eexists; repeat p; eauto.
+             econstructor; eauto.
+             eapply H5; eauto.
+             invert H40.
+             econstructor; eauto.
+             clean_map_lookups.
+           reflexivity.
+
+      + destruct (rec_u_id ==n u_id2); subst; clean_map_lookups; simpl in *.
+        * do 29 eexists; repeat p; eauto.
+             econstructor; eauto.
+             eapply H5; eauto.
+             invert H40.
+             econstructor; eauto.
+        * do 29 eexists; repeat p; eauto.
+             econstructor; eauto.
+             eapply H5; eauto.
+             invert H40.
+             econstructor; eauto.
+             clean_map_lookups.
+           reflexivity.
+
+    - split_ex; subst.
+      match goal with
+      | [ H : step_user _ (Some u_id2) _ _ |- _ ] => invert H; try contradiction
+      end; clean_map_lookups.
+      + do 29 eexists; repeat p; eauto.
+           econstructor; eauto.
+           eapply H2; eauto.
+      + do 29 eexists; repeat p; eauto.
+           destruct (k_id ==n k_id0); subst; econstructor; eauto.
+           eapply H2; eauto.
+      + do 29 eexists; repeat p; eauto.
+           destruct (k_id ==n k_id0); subst; econstructor; eauto.
+           eapply H2; eauto.
+
+    - split_ex; subst.
+      match goal with
+      | [ H : step_user _ (Some u_id2) _ _ |- _ ] => invert H; try contradiction
+      end; clean_map_lookups.
+      + do 29 eexists; repeat p; eauto.
+           econstructor; eauto.
+           eapply H2; eauto.
+      + do 29 eexists; repeat p; eauto.
+           destruct (k_id ==n k_id0); subst; econstructor; eauto.
+           eapply H2; eauto.
+      + do 29 eexists; repeat p; eauto.
+           destruct (k_id ==n k_id0); subst; econstructor; eauto.
+           eapply H2; eauto.
+  Qed.
+
+
+  Lemma commutes_sound'' :
+    forall {A B C} suid1 u_id1 lbl1 (bd1 bd1' : data_step0 A B C),
+
+      step_user lbl1 suid1 bd1 bd1'
+      -> suid1 = Some u_id1
+      -> forall bd2 bd2' lbl2 suid2 u_id2,
+
+          step_user lbl2 suid2 bd2 bd2'
+          -> suid2 = Some u_id2
+          -> u_id1 <> u_id2
+
+          -> forall cs1 cs1' cs1'' (usrs1 usrs1': honest_users A) (adv1 adv1' adv1'' : user_data B) gks1 gks1' gks1''
+              (cmd__n1 cmd__n1' : user_cmd C) ks1 ks1' qmsgs1 qmsgs1' mycs1 mycs1'
+              (cmd1 cmd1' cmd2 cmd2': user_cmd (Base A))
+              froms1 froms1' sents1 sents1' cur_n1 cur_n1'
+              usrs2 usrs2' ks2 ks2' qmsgs2 qmsgs2' mycs2 mycs2'
+              (* (cmd__n2 cmd__n2' : user_cmd D) *)
+              froms2 froms2' sents2 sents2' cur_n2 cur_n2' s,
+
+                bd1 = (usrs1, adv1, cs1, gks1, ks1, qmsgs1, mycs1, froms1, sents1, cur_n1, cmd__n1)
+              -> bd1' = (usrs1', adv1', cs1', gks1', ks1', qmsgs1', mycs1', froms1', sents1', cur_n1', cmd__n1')
+              -> bd2 = (usrs2, adv1', cs1', gks1', ks2, qmsgs2, mycs2, froms2, sents2, cur_n2, cmd2)
+              -> bd2' = (usrs2', adv1'', cs1'', gks1'', ks2', qmsgs2', mycs2', froms2', sents2', cur_n2', cmd2')
+
+              (* build link to overall user command *)
+              -> nextAction cmd1 cmd__n1
+              -> (forall r, cmd__n1 <> Return r)
+              -> (exists f, cmd1 = f cmd__n1
+                    /\ cmd1' = f cmd__n1'
+                    /\ forall lbl5 suid5 (usrs5 usrs5' : honest_users A) (adv5 adv5' : user_data B)
+                        cs5 cs5' gks5 gks5'
+                        ks5 ks5' qmsgs5 qmsgs5' mycs5 mycs5' (cmd__n'' : user_cmd C)
+                        froms5 froms5' sents5 sents5' cur_n5 cur_n5',
+
+                        step_user lbl5 suid5
+                                  (usrs5, adv5, cs5, gks5, ks5, qmsgs5, mycs5, froms5, sents5, cur_n5, cmd__n1)
+                                  (usrs5', adv5', cs5', gks5', ks5', qmsgs5', mycs5', froms5', sents5', cur_n5', cmd__n'')
+                        -> step_user lbl5 suid5
+                                    (usrs5, adv5, cs5, gks5, ks5, qmsgs5, mycs5, froms5, sents5, cur_n5, f cmd__n1)
+                                    (usrs5', adv5', cs5', gks5', ks5', qmsgs5', mycs5', froms5', sents5', cur_n5', f cmd__n'')
+
+                )
+              -> step_user lbl1 suid1
+                          (usrs1, adv1, cs1, gks1, ks1, qmsgs1, mycs1, froms1, sents1, cur_n1, cmd__n1)
+                          (usrs1', adv1', cs1', gks1', ks1', qmsgs1', mycs1', froms1', sents1', cur_n1', cmd__n1')
+
+              -> usrs1 $? u_id1 = Some (mkUserData ks1 cmd1 qmsgs1 mycs1 froms1 sents1 cur_n1)
+              -> usrs2 $? u_id2 = Some (mkUserData ks2 cmd2 qmsgs2 mycs2 froms2 sents2 cur_n2)
+              -> usrs2 = usrs1' $+ (u_id1, mkUserData ks1' cmd1' qmsgs1' mycs1' froms1' sents1' cur_n1')
+
+              -> summarize cmd1 s
+              -> commutes cmd2 s
+
+              -> forall bd3 ks3 qmsgs3 mycs3 froms3 sents3 cur_n3,
+                  bd3 = (usrs1, adv1, cs1, gks1, ks3, qmsgs3, mycs3, froms3, sents3, cur_n3, cmd2)
+                  -> usrs1 $? u_id2 = Some (mkUserData ks3 cmd2 qmsgs3 mycs3 froms3 sents3 cur_n3)
+                  
+                  -> exists bd3' lbl3 lbl4 bd4 bd4'
+                      cs3' (usrs3': honest_users A)
+                      (adv3' : user_data B) gks3'
+                      ks3' qmsgs3' mycs3' froms3' sents3' cur_n3'
+                      usrs4 usrs4' ks4 ks4' qmsgs4 qmsgs4' mycs4 mycs4'
+                      froms4 froms4' sents4 sents4' cur_n4 cur_n4',
+
+                      hstep lbl3 suid2 bd3 bd3'
+                      /\ bd3' = (usrs3', adv3', cs3', gks3', ks3', qmsgs3', mycs3', froms3', sents3', cur_n3', cmd2')
+                      /\ bd4 = (usrs4, adv3', cs3', gks3', ks4, qmsgs4, mycs4, froms4, sents4, cur_n4, cmd1)
+                      /\ bd4' = (usrs4', adv1'', cs1'', gks1'', ks4', qmsgs4', mycs4', froms4', sents4', cur_n4', cmd1')
+                      /\ usrs4 = usrs3' $+ (u_id2, mkUserData ks3' cmd2' qmsgs3' mycs3' froms3' sents3' cur_n3')
+                      /\ usrs4 $? u_id1 = Some (mkUserData ks4 cmd1 qmsgs4 mycs4 froms4 sents4 cur_n4)
+                      /\ hstep lbl4 suid1 bd4 bd4'
+  .
+  Proof.
+
+    intros.
+
+    Ltac p :=
+      match goal with
+      | [ |- _ /\ _ ] => simple apply conj
+      | [ |- _ = _ ] => reflexivity
+      | [ |- step_user _ _ _ _ ] => solve [ econstructor; repeat p; eauto ]
+      | [ H : ?m $+ (?k1,_) $? ?k2 = None |- ?m $? ?k3 = None ] =>
+        match type of m with
+        | keys => idtac
+        | ciphers => idtac
+        end;
+        is_not_evar k1; is_not_evar k2; is_evar k3; unify k3 k2;
+          destruct (k1 ==n k2); subst; clean_map_lookups; idtac 1
+      | [ H : ?m $+ (?k1,_) $? ?k2 = None |- ?m $+ (?k2,_) $? ?k3 = None ] =>
+        match type of m with
+        | keys => idtac
+        | ciphers => idtac
+        end;
+        is_not_evar k1; is_not_evar k2; is_evar k3; unify k3 k1;
+          destruct (k1 ==n k2); subst; clean_map_lookups; idtac 2
+      | [ |- (_,_) = _ ] => f_equal
+      | [ |- _ $+ (_,_) = _ ] => maps_equal
+      | [ |- _ $+ (_,_) $? _ = _ ] => clean_map_lookups
+      end.
+
+    Ltac simpl_solve uid :=
+      split_ex; subst;
+      match goal with
+      | [ H : step_user _ (Some uid) _ _ |- _ ] => invert H; try contradiction
+      end; clean_map_lookups;
+      do 29 eexists;
+         repeat p;
+         eauto;
+         repeat
+           match goal with
+           | [ |- hstep _ _ _ _ ] => solve [ econstructor; eauto ]
+           | [ H : forall _ _ _ _ _ _ _ _ _ _ _ _ _ _ _ _ _ _ _ _ _ _ _, step_user _ _ _ _  -> step_user _ _ _ _ |- hstep _ _ _ _ ] =>
+             solve [ eapply H; eauto ] 
+           end.
+         
+    induction 1; inversion 5; inversion 1; intros;
+      clean_context;
+      repeat 
+        match goal with
+        | [ H : (_,_,_,_,_,_,_,_,_,_,_) = (_,_,_,_,_,_,_,_,_,_,_) |- _ ] => invert H
+        | [ H : commutes _ _ |- _ ] => unfold commutes in H; try contradiction
+        end; clean_context; try (solve [ simpl_solve u_id2 ] ).
+
+
+    - apply nextAction_couldBe in H30; contradiction.
+    - split_ex; subst.
+      match goal with
+      | [ H : step_user _ (Some u_id2) _ _ |- _ ] => invert H; try contradiction
+      end; clean_map_lookups.
+      + destruct (rec_u_id ==n u_id2); subst; clean_map_lookups; simpl in *.
+        * do 29 eexists; repeat p; eauto.
+             econstructor; eauto.
+             eapply H5; eauto.
+             invert H40.
+             econstructor; eauto.
+        * do 29 eexists; repeat p; eauto.
+             econstructor; eauto.
+             eapply H5; eauto.
+             invert H40.
+             econstructor; eauto.
+             clean_map_lookups.
+             reflexivity.
+      + destruct (rec_u_id ==n u_id2); subst; clean_map_lookups; simpl in *.
+        * do 29 eexists; repeat p; eauto.
+             econstructor; eauto.
+             eapply H5; eauto.
+             invert H40.
+             econstructor; eauto.
+        * do 29 eexists; repeat p; eauto.
+             econstructor; eauto.
+             eapply H5; eauto.
+             invert H40.
+             econstructor; eauto.
+             clean_map_lookups.
+           reflexivity.
+
+      + destruct (rec_u_id ==n u_id2); subst; clean_map_lookups; simpl in *.
+        * do 29 eexists; repeat p; eauto.
+             econstructor; eauto.
+             eapply H5; eauto.
+             invert H40.
+             econstructor; eauto.
+        * do 29 eexists; repeat p; eauto.
+             econstructor; eauto.
+             eapply H5; eauto.
+             invert H40.
+             econstructor; eauto.
+             clean_map_lookups.
+           reflexivity.
+
+    - split_ex; subst.
+      match goal with
+      | [ H : step_user _ (Some u_id2) _ _ |- _ ] => invert H; try contradiction
+      end; clean_map_lookups.
+      + do 29 eexists; repeat p; eauto.
+           econstructor; eauto.
+           eapply H2; eauto.
+      + do 29 eexists; repeat p; eauto.
+           destruct (k_id ==n k_id0); subst; econstructor; eauto.
+           eapply H2; eauto.
+      + do 29 eexists; repeat p; eauto.
+           destruct (k_id ==n k_id0); subst; econstructor; eauto.
+           eapply H2; eauto.
+
+    - split_ex; subst.
+      match goal with
+      | [ H : step_user _ (Some u_id2) _ _ |- _ ] => invert H; try contradiction
+      end; clean_map_lookups.
+      + do 29 eexists; repeat p; eauto.
+           econstructor; eauto.
+           eapply H2; eauto.
+      + do 29 eexists; repeat p; eauto.
+           destruct (k_id ==n k_id0); subst; econstructor; eauto.
+           eapply H2; eauto.
+      + do 29 eexists; repeat p; eauto.
+           destruct (k_id ==n k_id0); subst; econstructor; eauto.
+           eapply H2; eauto.
+  Qed.
+
+
+
+
+
+
+
+  Require Import Coq.Program.Equality.
+  
+  Lemma commutes_sound' :
+    forall {A B} suid1 u_id1 lbl1 bd1 bd1',
+
+      hstep lbl1 suid1 bd1 bd1'
+      -> suid1 = Some u_id1
+      -> forall bd2 bd2' lbl2 suid2 u_id2,
+
+          hstep lbl2 suid2 bd2 bd2'
+          -> suid2 = Some u_id2
+          -> u_id1 <> u_id2
+
+          -> forall cs1 cs1' cs1'' (usrs1 usrs1': honest_users A) (adv1 adv1' adv1'' : user_data B) gks1 gks1' gks1''
+              cmd1 cmd1' ks1 ks1' qmsgs1 qmsgs1' mycs1 mycs1'
+              froms1 froms1' sents1 sents1' cur_n1 cur_n1'
+              usrs2 usrs2' cmd2 cmd2' ks2 ks2' qmsgs2 qmsgs2' mycs2 mycs2'
+              froms2 froms2' sents2 sents2' cur_n2 cur_n2' s,
+
+                bd1 = (usrs1, adv1, cs1, gks1, ks1, qmsgs1, mycs1, froms1, sents1, cur_n1, cmd1)
+              -> bd1' = (usrs1', adv1', cs1', gks1', ks1', qmsgs1', mycs1', froms1', sents1', cur_n1', cmd1')
+              -> bd2 = (usrs2, adv1', cs1', gks1', ks2, qmsgs2, mycs2, froms2, sents2, cur_n2, cmd2)
+              -> bd2' = (usrs2', adv1'', cs1'', gks1'', ks2', qmsgs2', mycs2', froms2', sents2', cur_n2', cmd2')
+
+              -> usrs1 $? u_id1 = Some (mkUserData ks1 cmd1 qmsgs1 mycs1 froms1 sents1 cur_n1)
+              -> usrs2 $? u_id2 = Some (mkUserData ks2 cmd2 qmsgs2 mycs2 froms2 sents2 cur_n2)
+              -> usrs2 = usrs1' $+ (u_id1, mkUserData ks1' cmd1' qmsgs1' mycs1' froms1' sents1' cur_n1')
+
+              -> summarize cmd1 s
+              -> commutes cmd2 s
+
+              -> forall bd3 ks3 qmsgs3 mycs3 froms3 sents3 cur_n3,
+                  bd3 = (usrs1, adv1, cs1, gks1, ks3, qmsgs3, mycs3, froms3, sents3, cur_n3, cmd2)
+                  -> usrs1 $? u_id2 = Some (mkUserData ks3 cmd2 qmsgs3 mycs3 froms3 sents3 cur_n3)
+                  
+                  -> exists bd3' lbl3 lbl4 bd4 bd4'
+                      cs3' (usrs3': honest_users A)
+                      (adv3' : user_data B) gks3'
+                      ks3' qmsgs3' mycs3' froms3' sents3' cur_n3'
+                      usrs4 usrs4' ks4 ks4' qmsgs4 qmsgs4' mycs4 mycs4'
+                      froms4 froms4' sents4 sents4' cur_n4 cur_n4',
+
+                      hstep lbl3 suid2 bd3 bd3'
+                      /\ usrs1 $? u_id2 = Some (mkUserData ks3 cmd2 qmsgs3 mycs3 froms3 sents3 cur_n3)
+                      /\ bd3' = (usrs3', adv3', cs3', gks3', ks3', qmsgs3', mycs3', froms3', sents3', cur_n3', cmd2')
+                      /\ bd4 = (usrs4, adv3', cs3', gks3', ks4, qmsgs4, mycs4, froms4, sents4, cur_n4, cmd1)
+                      /\ usrs4 = usrs3' $+ (u_id2, mkUserData ks3' cmd1' qmsgs3' mycs3' froms3' sents3' cur_n3')
+                      /\ usrs4 $? u_id1 = Some (mkUserData ks4 cmd1 qmsgs4 mycs4 froms4 sents4 cur_n4)
+                      /\ hstep lbl4 suid1 bd4 bd4'
+                      /\ bd4' = (usrs4', adv1'', cs1'', gks1'', ks4', qmsgs4', mycs4', froms4', sents4', cur_n4', cmd1')
+  .
+  Proof.
+    unfold hstep.
+
+    Hint Constructors step_user : core.
+    Hint Extern 1 (_ /\ _) => split : core.
+    Hint Extern 1 (_ = _) => reflexivity : core.
+
+    intros * STEP.
+    dependent induction STEP;
+      intros;
+      clean_context;
+      repeat 
+        match goal with
+        | [ H : (_,_,_,_,_,_,_,_,_,_,_) = _ |- _ ] => invert H
+        | [ H : commutes _ _ |- _ ] => unfold commutes in H; try contradiction
+        end.
+
+    Ltac p :=
+      match goal with
+      | [ |- _ /\ _ ] => simple apply conj
+      | [ |- _ = _ ] => reflexivity
+      | [ |- step_user _ _ _ _ ] => solve [ econstructor; repeat p; eauto ]
+      | [ H : ?m $+ (?k1,_) $? ?k2 = None |- ?m $? ?k3 = None ] =>
+        match type of m with
+        | keys => idtac
+        | ciphers => idtac
+        end;
+        is_not_evar k1; is_not_evar k2; is_evar k3; unify k3 k2;
+          destruct (k1 ==n k2); subst; clean_map_lookups; idtac 1
+      | [ H : ?m $+ (?k1,_) $? ?k2 = None |- ?m $+ (?k2,_) $? ?k3 = None ] =>
+        match type of m with
+        | keys => idtac
+        | ciphers => idtac
+        end;
+        is_not_evar k1; is_not_evar k2; is_evar k3; unify k3 k1;
+          destruct (k1 ==n k2); subst; clean_map_lookups; idtac 2
+      | [ |- (_,_) = _ ] => f_equal
+      | [ |- _ $+ (_,_) = _ ] => maps_equal
+      | [ |- _ $+ (_,_) $? _ = _ ] => clean_map_lookups
+      end.
+
+    shelve.
+    - clean_map_lookups.
+      invert H0. admit. admit. admit. admit. admit.
+
+    all : match goal with
+          | [ H : step_user _ _ _ _ |- _ ] => invert H; try contradiction
+          end; clean_map_lookups; do 29 eexists; repeat p.
+
+    Unshelve.
+
+    clean_map_lookups.
+    invert H10.
+
+    eapply IHSTEP in H0; clear IHSTEP; eauto.
+    shelve.
+    clear IHstep_user.
+    
+
+
+
+
+
+  
+
+  Lemma commutes_sound' :
+    forall {A B} suid1 u_id1 lbl1 bd1 bd1',
+
+      hstep lbl1 suid1 bd1 bd1'
+      -> suid1 = Some u_id1
+      -> forall bd2 bd2' lbl2 suid2 u_id2,
+
+          hstep lbl2 suid2 bd2 bd2'
+          -> suid2 = Some u_id2
+          -> u_id1 <> u_id2
+
+          -> forall cs1 cs1' cs1'' (usrs1 usrs1': honest_users A) (adv1 adv1' adv1'' : user_data B) gks1 gks1' gks1''
+              cmd1 cmd1' ks1 ks1' qmsgs1 qmsgs1' mycs1 mycs1'
+              froms1 froms1' sents1 sents1' cur_n1 cur_n1'
+              usrs2 usrs2' cmd2 cmd2' ks2 ks2' qmsgs2 qmsgs2' mycs2 mycs2'
+              froms2 froms2' sents2 sents2' cur_n2 cur_n2' s,
+
+                bd1 = (usrs1, adv1, cs1, gks1, ks1, qmsgs1, mycs1, froms1, sents1, cur_n1, cmd1)
+              -> bd1' = (usrs1', adv1', cs1', gks1', ks1', qmsgs1', mycs1', froms1', sents1', cur_n1', cmd1')
+              -> bd2 = (usrs2, adv1', cs1', gks1', ks2, qmsgs2, mycs2, froms2, sents2, cur_n2, cmd2)
+              -> bd2' = (usrs2', adv1'', cs1'', gks1'', ks2', qmsgs2', mycs2', froms2', sents2', cur_n2', cmd2')
+
+              -> usrs1 $? u_id1 = Some (mkUserData ks1 cmd1 qmsgs1 mycs1 froms1 sents1 cur_n1)
+              -> usrs2 $? u_id2 = Some (mkUserData ks2 cmd2 qmsgs2 mycs2 froms2 sents2 cur_n2)
+              -> usrs2 = usrs1' $+ (u_id1, mkUserData ks1' cmd1' qmsgs1' mycs1' froms1' sents1' cur_n1')
+
+              -> summarize cmd1 s
+              -> commutes cmd2 s
+
+              -> forall bd3 ks3 qmsgs3 mycs3 froms3 sents3 cur_n3,
+                  bd3 = (usrs1, adv1, cs1, gks1, ks3, qmsgs3, mycs3, froms3, sents3, cur_n3, cmd2)
+                  -> usrs1 $? u_id2 = Some (mkUserData ks3 cmd2 qmsgs3 mycs3 froms3 sents3 cur_n3)
+                  
+                  -> exists bd3' lbl3 lbl4 bd4 bd4'
+                      cs3' (usrs3': honest_users A)
+                      (adv3' : user_data B) gks3'
+                      ks3' qmsgs3' mycs3' froms3' sents3' cur_n3'
+                      usrs4 usrs4' ks4 ks4' qmsgs4 qmsgs4' mycs4 mycs4'
+                      froms4 froms4' sents4 sents4' cur_n4 cur_n4',
+
+                      hstep lbl3 suid2 bd3 bd3'
+                      /\ usrs1 $? u_id2 = Some (mkUserData ks3 cmd2 qmsgs3 mycs3 froms3 sents3 cur_n3)
+                      /\ bd3' = (usrs3', adv3', cs3', gks3', ks3', qmsgs3', mycs3', froms3', sents3', cur_n3', cmd2')
+                      /\ bd4 = (usrs4, adv3', cs3', gks3', ks4, qmsgs4, mycs4, froms4, sents4, cur_n4, cmd1)
+                      /\ usrs4 = usrs3' $+ (u_id2, mkUserData ks3' cmd1' qmsgs3' mycs3' froms3' sents3' cur_n3')
+                      /\ usrs4 $? u_id1 = Some (mkUserData ks4 cmd1 qmsgs4 mycs4 froms4 sents4 cur_n4)
+                      /\ hstep lbl4 suid1 bd4 bd4'
+                      /\ bd4' = (usrs4', adv1'', cs1'', gks1'', ks4', qmsgs4', mycs4', froms4', sents4', cur_n4', cmd1')
+  .
+  Proof.
+    unfold hstep.
+
+    Hint Constructors step_user : core.
+    Hint Extern 1 (_ /\ _) => split : core.
+    Hint Extern 1 (_ = _) => reflexivity : core.
+
+    intros * STEP.
+    dependent induction STEP;
+      intros;
+      clean_context;
+      repeat 
+        match goal with
+        | [ H : (_,_,_,_,_,_,_,_,_,_,_) = _ |- _ ] => invert H
+        | [ H : commutes _ _ |- _ ] => unfold commutes in H; try contradiction
+        end.
+
+    Ltac p :=
+      match goal with
+      | [ |- _ /\ _ ] => simple apply conj
+      | [ |- _ = _ ] => reflexivity
+      | [ |- step_user _ _ _ _ ] => solve [ econstructor; repeat p; eauto ]
+      | [ H : ?m $+ (?k1,_) $? ?k2 = None |- ?m $? ?k3 = None ] =>
+        match type of m with
+        | keys => idtac
+        | ciphers => idtac
+        end;
+        is_not_evar k1; is_not_evar k2; is_evar k3; unify k3 k2;
+          destruct (k1 ==n k2); subst; clean_map_lookups; idtac 1
+      | [ H : ?m $+ (?k1,_) $? ?k2 = None |- ?m $+ (?k2,_) $? ?k3 = None ] =>
+        match type of m with
+        | keys => idtac
+        | ciphers => idtac
+        end;
+        is_not_evar k1; is_not_evar k2; is_evar k3; unify k3 k1;
+          destruct (k1 ==n k2); subst; clean_map_lookups; idtac 2
+      | [ |- (_,_) = _ ] => f_equal
+      | [ |- _ $+ (_,_) = _ ] => maps_equal
+      | [ |- _ $+ (_,_) $? _ = _ ] => clean_map_lookups
+      end.
+
+    shelve.
+    
+    all : match goal with
+          | [ H : step_user _ _ _ _ |- _ ] => invert H; try contradiction
+          end; clean_map_lookups; do 29 eexists; repeat p.
+
+    Unshelve.
+
+    clean_map_lookups.
+    invert H10.
+
+    eapply IHSTEP in H0; clear IHSTEP; eauto.
+    shelve.
+    clear IHstep_user.
+    
+  Admitted.
+
+
+
+  
+  Lemma commutes_sound' :
+    forall {A B C}
+      suid1 u_id1 cs1 cs1' (usrs1 usrs1': honest_users A) (adv1 adv1' : user_data B) gks1 gks1' lbl1
+      ks1 ks1' qmsgs1 qmsgs1' mycs1 mycs1' froms1 froms1' sents1 sents1' cur_n1 cur_n1' bd1 bd1',
+
+      step_user lbl1 suid1 bd1 bd1'
+      -> suid1 = Some u_id1
+      -> bd1 = (usrs1, adv1, cs1, gks1, ks1, qmsgs1, mycs1, froms1, sents1, cur_n1, cmd1)
+      -> bd1' = (usrs1', adv1', cs1', gks1', ks1', qmsgs1', mycs1', froms1', sents1', cur_n1', cmd1')
+                     
+      -> forall suid2 u_id2 cs2 (usrs2 : honest_users A) (adv2 : user_data B) gks2 lbl2
+          ks2 qmsgs2 mycs2 froms2 sents2 cur_n2 bd2 s,
+
+          -> step_user lbl2 suid2 bd1' bd2
+          -> suid2 = Some u_id2
+          -> u_id1 <> u_id2
+          -> bd2 = (usrs2, adv2, cs2, gks2, ks2, qmsgs2, mycs2, froms2, sents2, cur_n2, cmd2)
+
+          -> forall cmdu1 cmdu2,
+              usrs1 $? u_id1 = Some {| key_heap  := ks1;
+                                       protocol  := cmdu1;
+                                       msg_heap  := qmsgs1;
+                                       c_heap    := mycs1;
+                                       from_nons := froms1;
+                                       sent_nons := sents1;
+                                       cur_nonce := cur_n1 |}
+              -> usrs1' $? u_id2 = Some {| key_heap  := ks1;
+                                          protocol  := cmdu1;
+                                          msg_heap  := qmsgs1;
+                                          c_heap    := mycs1;
+                                          from_nons := froms1;
+                                          sent_nons := sents1;
+                                          cur_nonce := cur_n1 |}
+
+          -> summarize cmd1 s
+          -> commutes cmd2 s
+          -> exists cs3 (usrs3 : honest_users A) (adv3 : user_data B) gks3 lbl3
+              ks3 qmsgs3 mycs3 froms3 sents3 cur_n3 bd3,
+              step_usr lbl3 suid2 bd3 bd3'
+              -> bd3 = (usrs1, adv1, cs1, gks1, ks1, qmsgs1, mycs1, froms1, sents1, cur_n1, cmd1)
+
+
+
+
+
+  
+
+
+  Lemma silent_commutes_nobind' :
+    forall {A B C} suid u_id cs cs' (usrs usrs': honest_users A)
+      (adv adv' : user_data B) gks gks' lbl
+      ks ks' qmsgs qmsgs' mycs mycs' froms froms' sents sents' cur_n cur_n' bd bd',
+
+      step_user lbl suid bd bd'
+      -> lbl = Silent
+      -> suid = Some u_id
+      -> forall (cmd cmd' : user_cmd C),
+          (* usrs $? u_id = Some {| key_heap  := ks; *)
+          (*                        protocol  := cmd; *)
+          (*                        msg_heap  := qmsgs; *)
+          (*                        c_heap    := mycs; *)
+          (*                        from_nons := froms; *)
+          (*                        sent_nons := sents; *)
+          (*                        cur_nonce := cur_n |} *)
+
+            bd = (usrs, adv, cs, gks, ks, qmsgs, mycs, froms, sents, cur_n, cmd)
+          -> bd' = (usrs', adv', cs', gks', ks', qmsgs', mycs', froms', sents', cur_n', cmd')
+          -> forall U__r U__r' U__i ud,
+              labels_align (U__r', U__i)
+              -> usrs $? u_id = Some ud
+              -> U__r = buildUniverse usrs adv cs gks u_id ud
+              -> U__r' = buildUniverse usrs' adv' cs' gks' u_id
+                                    {| key_heap  := ks';
+                                       protocol  := cmd';
+                                       msg_heap  := qmsgs';
+                                       c_heap    := mycs';
+                                       from_nons := froms';
+                                       sent_nons := sents';
+                                       cur_nonce := cur_n' |}
+              -> labels_align (U__r,U__i).
+  Proof.
+    induction 1.
+
+
+  
+  Infix "==" := JMeq (at level 70, no associativity).
+
+  Lemma silent_commutes' :
+    forall {A B C} suid u_id cs cs' (usrs usrs': honest_users A)
+      (adv adv' : user_data B) gks gks' lbl
+      ks ks' qmsgs qmsgs' mycs mycs' froms froms' sents sents' cur_n cur_n' bd bd',
+
+      step_user lbl suid bd bd'
+      -> lbl = Silent
+      -> suid = Some u_id
+      -> forall (cmdc cmdc' : user_cmd C) cmd cmd',
+          usrs $? u_id = Some {| key_heap  := ks;
+                                 protocol  := cmd;
+                                 msg_heap  := qmsgs;
+                                 c_heap    := mycs;
+                                 from_nons := froms;
+                                 sent_nons := sents;
+                                 cur_nonce := cur_n |}
+
+          -> bd = (usrs, adv, cs, gks, ks, qmsgs, mycs, froms, sents, cur_n, cmdc)
+          -> bd' = (usrs', adv', cs', gks', ks', qmsgs', mycs', froms', sents', cur_n', cmdc')
+          (* -> (C = Base A /\ cmdc = cmd) *)
+          -> (cmd == cmdc \/ exists cmdcc, cmd = Bind cmdc cmdcc)
+          -> forall U__r U__r' U__i ud,
+              labels_align (U__r', U__i)
+              -> usrs $? u_id = Some ud
+              -> U__r = buildUniverse usrs adv cs gks u_id ud
+              -> U__r' = buildUniverse usrs' adv' cs' gks' u_id
+                                    {| key_heap  := ks';
+                                       protocol  := cmd';
+                                       msg_heap  := qmsgs';
+                                       c_heap    := mycs';
+                                       from_nons := froms';
+                                       sent_nons := sents';
+                                       cur_nonce := cur_n' |}
+              -> labels_align (U__r,U__i).
+  Proof.
+    induction 1; inversion 4; inversion 1; intros; subst; intros;
+      try discriminate;
+      clean_context;
+      eauto 8.
+
+    admit.
+    admit.
+
+    split_ors.
+    inversion H.
+    generalize (JMeq_eq H).
+    
+    
+    
+  Admitted.
+                                  
+  Lemma silent_commutes :
+    forall {A B} (U__r U__r' : universe A B) (U__i : IdealWorld.universe A) b,
+      step_universe U__r Silent U__r'
+      -> lameAdv b U__r.(adversary)
+      -> labels_align (U__r',U__i)
+      -> labels_align (U__r ,U__i).
+  Proof.
+    intros.
+    invert H; destruct U__r; simpl in *.
+    - destruct userData; simpl in *.
+      eapply silent_commutes'; eauto.
+      reflexivity.
+      unfold buildUniverse; simpl.
+      f_equal.
+      maps_equal.
+
+    - unfold lameAdv, build_data_step in *; simpl in *.
+      rewrite H0 in *.
+      invert H2.
+  Qed.
+
+
+
 
   Inductive UVal (t : user_cmd_type) : Set :=
   | ConcreteVal (v : << t >> )
@@ -162,7 +1491,7 @@ Section RealWorldLemmas.
 
   (*
    * And that the syntactic safety predicate is preserved through any
-   * silent real world step 
+   * silent real world step
    *)
   Lemma syntactically_safe_preservation' :
     forall {A B} (U U': universe A B),
@@ -177,7 +1506,7 @@ Section RealWorldLemmas.
 
 
 
-      
+
     - admit.  (* assume adversary cannot step, in lame world! *)
 
   Admitted.
@@ -237,5 +1566,5 @@ Module Gen (PD : ProcDef).
    * Now, I want to use all of the above lemmas to prove simulation, essentially converting
    * the whole proof into the above syntactic protocol check, plus some labeled step verification.
    *)
-  
+
 End Gen.
